Add patterns "constrained_since" and "dual_constrained_since", rename patterns and lemmas? remove proof methods.

Constrained_Until.thy
@@ -1,25 +1,25 @@
 theory Constrained_Until
-  imports Previous
+  imports RequirementLemmas
 begin
 
-definition constrained_until where "constrained_until t A1 A2  s s1 \<equiv>
+definition constrained_until0 where "constrained_until0 t A1 A2 s s1 \<equiv>
 toEnvNum s1 s \<ge> t \<longrightarrow>
 (\<exists> r2. toEnvP r2 \<and> s1 \<le> r2 \<and> r2 \<le> s \<and> toEnvNum s1 r2 \<le> t \<and> A2 s r2 \<and>
 (\<forall> r1. toEnvP r1 \<and> s1 \<le> r1 \<and> r1 < r2 \<longrightarrow> A1 s r1))"
 
-definition constrained_until_inv where "constrained_until_inv  t t1 A1' A2' s s1 \<equiv>
+definition constrained_until0_inv where "constrained_until0_inv  t t1 A1' A2' s s1 \<equiv>
 (\<exists> r2. toEnvP r2 \<and> s1 \<le> r2 \<and> r2 \<le> s \<and> toEnvNum s1 r2 \<le> t \<and> A2' s r2 \<and>
 (\<forall> r1. toEnvP r1 \<and> s1 \<le> r1 \<and> r1 < r2 \<longrightarrow> A1' s r1)) \<or>
 toEnvNum s1 s < t1 s \<and>
 (\<forall> r1. toEnvP r1 \<and> s1 \<le> r1 \<and> r1 \<le> s \<longrightarrow> A1' s r1)"
 
-lemma constrained_until_rule[patternintro]: "
+lemma constrained_until0_L1: "
 consecutive s s' \<Longrightarrow>
 always_imp s (A1' s) (A1' s') \<and>
 always_imp s (A2' s) (A2' s') \<and>
  (t1 s = 0 \<or> A2' s' s' \<and> t1 s \<le> t \<or> A1' s' s' \<and> t1 s < t1 s') \<Longrightarrow>
-always_imp s (\<lambda> s1. constrained_until_inv t t1 A1' A2' s s1) (\<lambda> s1. constrained_until_inv t t1 A1' A2' s' s1)"
-  apply(unfold constrained_until_inv_def always_imp_def)
+always_imp s (\<lambda> s1. constrained_until0_inv t t1 A1' A2' s s1) (\<lambda> s1. constrained_until0_inv t t1 A1' A2' s' s1)"
+  apply(unfold constrained_until0_inv_def always_imp_def)
     unfolding less_eq_state.simps less_state.simps
   apply(rule allI)
   subgoal for s1
@@ -49,38 +49,38 @@ always_imp s (\<lambda> s1. constrained_until_inv t t1 A1' A2' s s1) (\<lambda> 
     by (smt (verit, ccfv_SIG) consecutive.elims(2) less_imp_add_positive less_numeral_extra(3) less_one linorder_neqE_nat nat_add_left_cancel_less substate_noteq_imp_substate_of_pred trans_less_add1 zero_less_one)
   done
 
-lemma constrained_until_einv2req[patternintro]: "
+lemma constrained_until0_L2: "
+toEnvP s \<Longrightarrow>A2' s s \<or> A1' s s \<and> t1 s > 0 \<Longrightarrow> constrained_until0_inv t t1 A1' A2' s s"
+  unfolding constrained_until0_inv_def always_imp_def
+  by (metis bot_nat_0.extremum dual_order.refl leD order_le_imp_less_or_eq toEnvNum_id)
+
+lemma constrained_until0_L3: "
 toEnvP s \<Longrightarrow>
 always_imp s (A1' s) (A1 s) \<and>
 always_imp s (A2' s) (A2 s) \<and>
 t1 s \<le> t \<Longrightarrow>
-always_imp s (\<lambda> s1. constrained_until_inv t t1 A1' A2' s s1) (\<lambda> s1. constrained_until  t A1 A2 s s1)"
-  unfolding constrained_until_inv_def constrained_until_def always_imp_def less_eq_state.simps less_state.simps
+always_imp s (\<lambda> s1. constrained_until0_inv t t1 A1' A2' s s1) (\<lambda> s1. constrained_until0  t A1 A2 s s1)"
+  unfolding constrained_until0_inv_def constrained_until0_def always_imp_def less_eq_state.simps less_state.simps
   by (metis dual_order.trans substate_trans verit_comp_simplify1(3))
 
-lemma constrained_until_one_point[patternintro]: "
-toEnvP s \<Longrightarrow>A2' s s \<or> A1' s s \<and> t1 s > 0 \<Longrightarrow> constrained_until_inv t t1 A1' A2' s s"
-  unfolding constrained_until_inv_def always_imp_def
-  by (metis bot_nat_0.extremum dual_order.refl leD order_le_imp_less_or_eq toEnvNum_id)
-
-definition constrained_until2 where "constrained_until2 t1 t2 A1 A2  s s1 \<equiv>
+definition constrained_until where "constrained_until t1 t2 A1 A2  s s1 \<equiv>
 toEnvNum s1 s \<ge> t2 \<longrightarrow>
 (\<exists> r2. toEnvP r2 \<and> s1 \<le> r2 \<and> r2 \<le> s \<and> toEnvNum s1 r2 \<ge> t1 \<and> toEnvNum s1 r2 \<le> t2 \<and> A2 s r2 \<and>
 (\<forall> r1. toEnvP r1 \<and> s1 \<le> r1 \<and> r1 < r2 \<longrightarrow> A1 s r1))"
 
-definition constrained_until2_inv where "constrained_until2_inv  t1 t2 t1_1 t2_1 A1' A2' s s1 \<equiv>
+definition constrained_until_inv where "constrained_until_inv  t1 t2 t1_1 t2_1 A1' A2' s s1 \<equiv>
 (\<exists> r2. toEnvP r2 \<and> s1 \<le> r2 \<and> r2 \<le> s \<and> toEnvNum s1 r2 \<ge> t1 \<and> toEnvNum s1 r2 \<le> t2 \<and> A2' s r2 \<and>
 (\<forall> r1. toEnvP r1 \<and> s1 \<le> r1 \<and> r1 < r2 \<longrightarrow> A1' s r1)) \<or>
 toEnvNum s1 s \<ge> t1_1 s \<and> toEnvNum s1 s < t2_1 s \<and>
 (\<forall> r1. toEnvP r1 \<and> s1 \<le> r1 \<and> r1 \<le> s \<longrightarrow> A1' s r1)"
 
-lemma constrained_until2_rule: "
+lemma constrained_until_L1: "
 consecutive s s' \<Longrightarrow>
 always_imp s (A1' s) (A1' s') \<and>
 always_imp s (A2' s) (A2' s') \<and>
  (t2_1 s = 0 \<or> t1_1 s \<ge> t2_1 s \<or> A2' s' s' \<and> t1_1 s + 1 \<ge> t1 \<and> t2_1 s \<le> t2 \<or> A1' s' s' \<and> t1_1 s + 1 \<ge> t1_1 s' \<and> t2_1 s < t2_1 s') \<Longrightarrow>
-always_imp s (\<lambda> s1. constrained_until2_inv t1 t2 t1_1 t2_1 A1' A2' s s1) (\<lambda> s1. constrained_until2_inv t1 t2 t1_1 t2_1 A1' A2' s' s1)"
-  apply(unfold constrained_until2_inv_def always_imp_def)
+always_imp s (\<lambda> s1. constrained_until_inv t1 t2 t1_1 t2_1 A1' A2' s s1) (\<lambda> s1. constrained_until_inv t1 t2 t1_1 t2_1 A1' A2' s' s1)"
+  apply(unfold constrained_until_inv_def always_imp_def)
     unfolding less_eq_state.simps less_state.simps
     apply(rule allI)
   subgoal for s1
@@ -117,19 +117,19 @@ always_imp s (\<lambda> s1. constrained_until2_inv t1 t2 t1_1 t2_1 A1' A2' s s1)
     by (smt (verit, ccfv_SIG) consecutive.elims(2) less_imp_add_positive less_numeral_extra(3) less_one linorder_neqE_nat nat_add_left_cancel_less substate_noteq_imp_substate_of_pred trans_less_add1 zero_less_one)
   done
 
-lemma constrained_until2_einv2req: "
+lemma constrained_until_L2: "
+toEnvP s \<Longrightarrow>t1 = 0 \<and>A2' s s \<or> A1' s s \<and> t1_1 s = 0 \<and> t2_1 s > 0 \<Longrightarrow> constrained_until_inv t1 t2 t1_1 t2_1 A1' A2' s s"
+  unfolding constrained_until_inv_def always_imp_def
+  by (metis bot_nat_0.extremum dual_order.refl leD order_le_imp_less_or_eq toEnvNum_id)
+
+lemma constrained_until_L3: "
 toEnvP s \<Longrightarrow>
 always_imp s (A1' s) (A1 s) \<and>
 always_imp s (A2' s) (A2 s) \<and>
 t2_1 s \<le> t2 \<Longrightarrow>
-always_imp s (\<lambda> s1. constrained_until2_inv t1 t2 t1_1 t2_1 A1' A2' s s1) (\<lambda> s1. constrained_until2  t1 t2 A1 A2 s s1)"
-  unfolding constrained_until2_inv_def constrained_until2_def always_imp_def less_eq_state.simps less_state.simps
+always_imp s (\<lambda> s1. constrained_until_inv t1 t2 t1_1 t2_1 A1' A2' s s1) (\<lambda> s1. constrained_until  t1 t2 A1 A2 s s1)"
+  unfolding constrained_until_inv_def constrained_until_def always_imp_def less_eq_state.simps less_state.simps
   by (metis dual_order.trans substate_trans verit_comp_simplify1(3))
-
-lemma constrained_until2_one_point: "
-toEnvP s \<Longrightarrow>t1 = 0 \<and>A2' s s \<or> A1' s s \<and> t1_1 s = 0 \<and> t2_1 s > 0 \<Longrightarrow> constrained_until2_inv t1 t2 t1_1 t2_1 A1' A2' s s"
-  unfolding constrained_until2_inv_def always_imp_def
- by (metis bot_nat_0.extremum dual_order.refl leD order_le_imp_less_or_eq toEnvNum_id)
 
 end
  
