EDTL_Low_Steady.thy
@@ -4,7 +4,7 @@ begin
 
 fun low_steady_time :: "state \<Rightarrow> (state \<Rightarrow> bool) \<Rightarrow> nat" where
 "low_steady_time emptyState A = 0" |
-"low_steady_time (toEnv s) A = (if \<not> A (toEnv s) then if prev s = emptyState \<or> A (prev s) then 0 else Suc (low_steady_time s A) else low_steady_time s A)" |
+"low_steady_time (toEnv s) A = (if \<not> A (toEnv s) then if prev (toEnv s) = emptyState \<or> A (prev (toEnv s)) then 0 else Suc (low_steady_time s A) else low_steady_time s A)" |
 "low_steady_time (setVarBool s x u) A = low_steady_time s A" |
 "low_steady_time (setVarInt s x u) A = low_steady_time s A" |
 "low_steady_time (setVarReal s x u) A = low_steady_time s A" |
@@ -21,8 +21,25 @@ A s1 \<and>
   (\<forall> s3. toEnvP s3 \<and> s3 \<le> s1 \<and> \<not> A s3 \<and> (\<forall> s4. toEnvP s4 \<and> s3 < s4 \<and> s4 \<le> s1 \<longrightarrow> A s4) \<longrightarrow> 
     ((\<exists> s2. toEnvP s2 \<and> s2 \<le> s3 \<and> toEnvNum s2 s3 \<le> t + 1 \<and> A s2) \<or> toEnvNum emptyState s3 \<le> t + 1 \<and> (\<forall> s2. toEnvP s2 \<and> s2 \<le> s3 \<longrightarrow> \<not> A s2)))"
 
+definition low_steady_upper_time_limit_if_false where "low_steady_upper_time_limit_if_false t A s s1 \<equiv>
+\<not> A s1 \<and> 
+  ((\<exists> s2. toEnvP s2 \<and> s2 \<le> s1 \<and> toEnvNum s2 s1 \<le> t + 1 \<and> A s2) \<or> toEnvNum emptyState s1 \<le> t + 1 \<and> (\<forall> s2. toEnvP s2 \<and> s2 \<le> s1 \<longrightarrow> \<not> A s2))"
+
+definition low_steady_upper_time_limit_if_true where "low_steady_upper_time_limit_if_true t A s s1 \<equiv>
+A s1 \<and>
+  (\<forall> s3. toEnvP s3 \<and> s3 \<le> s1 \<and> \<not> A s3 \<and> (\<forall> s4. toEnvP s4 \<and> s3 < s4 \<and> s4 \<le> s1 \<longrightarrow> A s4) \<longrightarrow> 
+    ((\<exists> s2. toEnvP s2 \<and> s2 \<le> s3 \<and> toEnvNum s2 s3 \<le> t + 1 \<and> A s2) \<or> toEnvNum emptyState s3 \<le> t + 1 \<and> (\<forall> s2. toEnvP s2 \<and> s2 \<le> s3 \<longrightarrow> \<not> A s2)))"
+
 definition low_steady_lower_time_limit where "low_steady_lower_time_limit t A s s1 \<equiv>
 \<not> A s1 \<and> toEnvNum emptyState s1 \<ge> t+1 \<and> (\<forall> s2. toEnvP s2 \<and> s2 \<le> s1 \<and> toEnvNum s2 s1 \<le> t \<longrightarrow> \<not> A s2) \<or>
+A s1 \<and> 
+  (\<exists> s3. toEnvP s3 \<and> s3 \<le> s1 \<and> (\<forall> s4. toEnvP s4 \<and> s3 < s4 \<and> s4 \<le> s1 \<longrightarrow> A s4) \<and>
+    toEnvNum emptyState s3 \<ge> t+1 \<and> (\<forall> s2. toEnvP s2 \<and> s2 \<le> s3 \<and> toEnvNum s2 s3 \<le> t \<longrightarrow> \<not> A s2))"
+
+definition low_steady_lower_time_limit_if_false where "low_steady_lower_time_limit_if_false t A s s1 \<equiv>
+\<not> A s1 \<and> toEnvNum emptyState s1 \<ge> t+1 \<and> (\<forall> s2. toEnvP s2 \<and> s2 \<le> s1 \<and> toEnvNum s2 s1 \<le> t \<longrightarrow> \<not> A s2)"
+
+definition low_steady_lower_time_limit_if_true where "low_steady_lower_time_limit_if_true t A s s1 \<equiv>
 A s1 \<and> 
   (\<exists> s3. toEnvP s3 \<and> s3 \<le> s1 \<and> (\<forall> s4. toEnvP s4 \<and> s3 < s4 \<and> s4 \<le> s1 \<longrightarrow> A s4) \<and>
     toEnvNum emptyState s3 \<ge> t+1 \<and> (\<forall> s2. toEnvP s2 \<and> s2 \<le> s3 \<and> toEnvNum s2 s3 \<le> t \<longrightarrow> \<not> A s2))"
